% 10.
\section{}

% 10.a.
\subsection{}
\begin{align*}
    Ac
    &= \begin{bmatrix}
	0 & 2 & 4 \\
	2 & 4 & 2 \\
	3 & 3 & 1
    \end{bmatrix}
    \begin{bmatrix}
	1 \\
	1 \\
	1
    \end{bmatrix} \\
    %
    &= \begin{bmatrix}
	1 * 0 + 1 * 2 + 1 * 4 \\
	1 * 2 + 1 * 4 + 1 * 2 \\
	1 * 3 + 1 * 3 + 1 * 1
    \end{bmatrix} \\
    %
    &= \begin{bmatrix}
	6 \\
	8 \\
	7
    \end{bmatrix}
\end{align*}

% 10.b.
\subsection{}
Find A$^{-1}$.
\begin{align*}
    A^{-1}
    &= \left[\begin{array}{ccc|ccc}
	0 & 2 & 4 & 1 & 0 & 0 \\
	2 & 4 & 2 & 0 & 1 & 0 \\
	3 & 3 & 1 & 0 & 0 & 1
    \end{array}\right] \\
    % 
    &= \left[\begin{array}{ccc|ccc}
	2 & 4 & 2 & 0 & 1 & 0 \\
	0 & 2 & 4 & 1 & 0 & 0 \\
	3 & 3 & 1 & 0 & 0 & 1
    \end{array}\right] \tag*{R1 $\Leftrightarrow$ R2} \\
    % 
    &= \left[\begin{array}{ccc|ccc}
	1 & 2 & 1 & 0 & \frac{1}{2} & 0 \\
	0 & 2 & 4 & 1 & 0 & 0 \\
	3 & 3 & 1 & 0 & 0 & 1
    \end{array}\right] \tag*{$\frac{R1}{2} \Rightarrow$ R1} \\
    % 
    &= \left[\begin{array}{ccc|ccc}
	1 & 2 & 1 & 0 & \frac{1}{2} & 0 \\
	0 & 2 & 4 & 1 & 0 & 0 \\
	0 & -3 & -2 & 0 & \frac{-3}{2} & 1
    \end{array}\right] \tag*{R3 - 3R1 $\Rightarrow$ R3} \\
    % 
    &= \left[\begin{array}{ccc|ccc}
	1 & 0 & -3 & -1 & \frac{1}{2} & 0 \\
	0 & 2 & 4 & 1 & 0 & 0 \\
	0 & -3 & -2 & 0 & \frac{-3}{2} & 1
    \end{array}\right] \tag*{R1 - R2 $\Rightarrow$ R1} \\
    % 
    &= \left[\begin{array}{ccc|ccc}
	1 & 0 & -3 & -1 & \frac{1}{2} & 0 \\
	0 & 1 & 2 & \frac{1}{2} & 0 & 0 \\
	0 & -3 & -2 & 0 & \frac{-3}{2} & 1
    \end{array}\right] \tag*{$\frac{R2}{2} \Rightarrow$ R1} \\
    % 
    &= \left[\begin{array}{ccc|ccc}
	1 & 0 & -3 & -1 & \frac{1}{2} & 0 \\
	0 & 1 & 2 & \frac{1}{2} & 0 & 0 \\
	0 & 0 & 4 & \frac{3}{2} & \frac{-3}{2} & 1
    \end{array}\right] \tag*{3R2 + R3 $\Rightarrow$ R3} \\
    % 
    &= \left[\begin{array}{ccc|ccc}
	1 & 0 & -3 & -1 & \frac{1}{2} & 0 \\
	0 & 1 & 2 & \frac{1}{2} & 0 & 0 \\
	0 & 0 & 1 & \frac{3}{8} & \frac{-3}{8} & \frac{1}{4}
    \end{array}\right] \tag*{$\frac{R3}{4} \Rightarrow$ R3} \\
    % 
    &= \left[\begin{array}{ccc|ccc}
	1 & 0 & 0 & \frac{1}{8} & \frac{-5}{8} & \frac{3}{4} \\
	0 & 1 & 2 & \frac{1}{2} & 0 & 0 \\
	0 & 0 & 1 & \frac{3}{8} & \frac{-3}{8} & \frac{1}{4}
    \end{array}\right] \tag*{3R3 + R1 $\Rightarrow$ R1} \\
    % 
    &= \left[\begin{array}{ccc|ccc}
	1 & 0 & 0 & \frac{1}{8} & \frac{-5}{8} & \frac{3}{4} \\
	0 & 1 & 0 & \frac{-1}{4} & \frac{3}{4} & \frac{-1}{2} \\
	0 & 0 & 1 & \frac{3}{8} & \frac{-3}{8} & \frac{1}{4}
    \end{array}\right] \tag*{-2R3 + R2 $\Rightarrow$ R2} \\
    % 
    &= \left[\begin{array}{ccc}
	\frac{1}{8} & \frac{-5}{8} & \frac{3}{4} \\
	\frac{-1}{4} & \frac{3}{4} & \frac{-1}{2} \\
	\frac{3}{8} & \frac{-3}{8} & \frac{1}{4}
    \end{array}\right]    
\end{align*}

Find x = A$^{-1}$B.
\begin{align*}
    x
    &= A^{-1}B \\
    %
    &= \begin{bmatrix}
	\frac{1}{8} & \frac{-5}{8} & \frac{3}{4} \\
	\frac{-1}{4} & \frac{3}{4} & \frac{-1}{2} \\
	\frac{3}{8} & \frac{-3}{8} & \frac{1}{4}
    \end{bmatrix}
    \begin{bmatrix}
	-2 \\
	-2 \\
	-4
    \end{bmatrix} \\
    %
    &= \begin{bmatrix}
	-2 * \frac{1}{8} -2 * \frac{-5}{8} -4 * \frac{3}{4} \\
	-2 * \frac{-1}{4} -2 * \frac{3}{4} -4 * \frac{-1}{2} \\
	-2 * \frac{3}{8} -2 * \frac{-3}{8} -4 * \frac{1}{4}
    \end{bmatrix} \\
    %
    &= \begin{bmatrix}
	-2 \\
	1 \\
	-1
    \end{bmatrix}
\end{align*}
