% 2.
\section{}

% 2.a.
\subsection{}

Show that if $E[Y|X=x]=x$ that $Cov(X, Y) = E[(X - E[X])^2]$.
\begin{align*}
    Cov(X, Y) &= E[X, Y] - E[X]E[Y] \\
	&= \sum_x P(X=x) E[XY | X] \\
	&= \sum_x P(X=x) x E[Y | X] \\
	&= \sum_x P(X=x) x^2 \tag*{Law of total expectation}\\
	&= E[X^2] - E[X]E[Y] \\
	&= E[X^2] - E[X] \sum_x P(X=x) E[Y | X=x] \\
	&= E[X^2] - E[X] \sum_x P(X=x) x \\
	&= E[X^2] - E[X]E[X] \tag*{Law of total expectation} \\
	&= E[X^2] - E[X]^2 \\
	&= E[(X - E[X])^2]
\end{align*}

% 2.b.
\subsection{}

Show that if X and Y are independent that $Cov(X, Y) = 0$.
\begin{align*}
Cov(X,Y)
    &= E[(X - E[X])(Y - E[Y])] \\
    &= E[XY] - E[X]E[Y] \\
    &= \sum_{x,y}P(X=x, Y=y) xy  - E[X]E[Y] \\
    &= \sum_{x,y}P(X=x)P(Y=y) xy  - E[X]E[Y] \\
    &= (\sum_x P(X=x) x) (\sum_y P(Y=y) y) - E[X]E[Y] \\
    &= E[X]E[Y] - E[X]E[Y] \\
    &= 0 \\ 
\end{align*}
