% 9.
\section{}

% 9.a.
\subsection{}
Write A in row echelon form.
\begin{align*}
    A
    &= \begin{bmatrix}
	1 & 2 & 1 \\
	1 & 0 & 3 \\
	1 & 1 & 2
    \end{bmatrix} \\
    %
    &= \begin{bmatrix}
	1 & 2 & 1 \\
	0 & -2 & 2 \\
	1 & 1 & 2
    \end{bmatrix} \tag*{R2 - R1 $\Rightarrow$ R2} \\
    %
    &= \begin{bmatrix}
	1 & 2 & 1 \\
	0 & -2 & 2 \\
	0 & -1 & 1
    \end{bmatrix} \tag*{R3 - R1 $\Rightarrow$ R3} \\
    %
    &= \begin{bmatrix}
	1 & 0 & 3 \\
	0 & -2 & 2 \\
	0 & -1 & 1
    \end{bmatrix} \tag*{R1 + R2 $\Rightarrow$ R1} \\
    %
    &= \begin{bmatrix}
	1 & 0 & 3 \\
	0 & -1 & 1 \\
	0 & -1 & 1
    \end{bmatrix} \tag*{$\frac{R2}{2} \Rightarrow$ R2} \\
    %
    &= \begin{bmatrix}
	1 & 0 & 3 \\
	0 & -1 & 1 \\
	0 & 0 & 0
    \end{bmatrix} \tag*{R2 + R3 $\Rightarrow$ R3}
\end{align*}
Since there are two nonzero rows in ref(A), rank(A)=2.

Write B in row echelon from.
\begin{align*}
    B 
    &= \begin{bmatrix}
	1 & 2 & 3 \\
	1 & 0 & 1 \\
	1 & 1 & 2
    \end{bmatrix} \\
    %
    &= \begin{bmatrix}
	1 & 2 & 3 \\
	0 & -2 & -2 \\
	1 & 1 & 2
    \end{bmatrix} \tag*{R2 - R1 $\Rightarrow$ R2} \\
    %
    &= \begin{bmatrix}
	1 & 2 & 3 \\
	0 & -2 & -2 \\
	0 & -1 & -1
    \end{bmatrix} \tag*{R3 - R1 $\Rightarrow$ R3} \\
    %
    &= \begin{bmatrix}
	1 & 2 & 3 \\
	0 & -1 & -1 \\
	0 & -1 & -1
    \end{bmatrix} \tag*{$\frac{R2}{2} \Rightarrow$ R2} \\
    %
    &= \begin{bmatrix}
	1 & 2 & 3 \\
	0 & -1 & -1 \\
	0 & 0 & 0
    \end{bmatrix} \tag*{R1 - R2 $\Rightarrow$ R3} 
\end{align*}
Since there are two nonzero rows in ref(B), rank(B)=2.

% 9.b.
\subsection{}
Since there are two pivot columns in ref(A), basis(A)=2.
\\
Since there are two pivot columns in ref(B), basis(B)=2.
