\begin{itemize}
    \item {\bf I is convex} on $[a, c]$.
    \item {\bf II is not convex} on $[a, d]$ because $f(\lambda c + (1 - \lambda) d) \geq \lambda f(c) + (1 - \lambda) f(d)$ on $[c, d]$ for an arbitrary $\lambda$.
    \item {\bf II is convex} on $[a, b]$.
    \item {\bf III is not convex} on $[a, c]$ because $f(\lambda a + (1 - \lambda) b) \geq \lambda f(a) + (1 - \lambda) f(b)$ on $[a, b]$ and $f(\lambda b + (1 - \lambda) c) \geq \lambda f(b) + (1 - \lambda) f(c)$ on $[b, c]$ for an arbitrary $\lambda$.
\end{itemize}
